test_seccomp.ml
@@ -1,5 +1,5 @@
 open Seccomp
-open Seccompjit
+open Seccompfilter
 open AST
 open PrintCminor
 open Errors
@@ -17,7 +17,7 @@ let print_error oc msg =
 
 let jit_and_print f =
   let p = { prog_defs = [(P.one, Gfun (Internal f))]; prog_main = P.one } in
-  match Seccompjit.transl_program p with
+  match Seccompfilter.transl_program_filter p with
   | Errors.OK x -> print_program (Format.formatter_of_out_channel stdout) x
   | Errors.Error msg -> print_error stdout msg
     (* using stdout instead of stderr to fully order diagnostic output *)
@@ -31,6 +31,7 @@ in List.map jit_and_print [
     Seccomp.Sjmp_ja Integers.Int.zero;
     Seccomp.Sjmp_ja Integers.Int.one;
     Seccomp.Salu_safe (Aaddimm Integers.Int.one);
+    Seccomp.Sjmp_ja Integers.Int.one;
     Seccomp.Sret_a;
   ];
   [
