codegen/extraction.v
@@ -3,11 +3,12 @@ Require Import ExtrOcamlString.
 Require Import Seccomp.
 Require Import Seccompjit.
 Require Import Seccompenc.
+Require Import Seccompfilter.
 Require Import compcert.common.Errors.
 
 Extraction Blacklist List String Int.
 
-Extraction Inline Errors.bind Errors.bind2.
+Extraction Inline Errors.bind Errors.bind2 List.last.
 
 Extract Constant AST.ident_of_string =>
   "fun s -> Camlcoq.intern_string (Camlcoq.camlstring_of_coqstring s)".
@@ -22,3 +23,4 @@ Cd "codegen".
 Extraction Library Seccomp.
 Extraction Library Seccompjit.
 Extraction Library Seccompenc.
+Extraction Library Seccompfilter.
